theories/Core/Semantic/Evaluation/Definitions.v
@@ -2,85 +2,90 @@ From Mcltt Require Import Base.
 From Mcltt Require Export Domain.
 Import Domain_Notations.
 
-Reserved Notation "'⟦' M '⟧' p '↘' r" (in custom judg at level 80, M custom exp at level 99, p custom domain at level 99, r custom domain at level 99).
-Reserved Notation "'rec' m '⟦return' A | 'zero' -> MZ | 'succ' -> MS 'end⟧' p '↘' r" (in custom judg at level 80, m custom domain at level 99, A custom exp at level 99, MZ custom exp at level 99, MS custom exp at level 99, p custom domain at level 99, r custom domain at level 99).
+Reserved Notation "'⟦' M '⟧' ρ '↘' r" (in custom judg at level 80, M custom exp at level 99, ρ custom domain at level 99, r custom domain at level 99).
+Reserved Notation "'rec' m '⟦return' A | 'zero' -> MZ | 'succ' -> MS 'end⟧' ρ '↘' r" (in custom judg at level 80, m custom domain at level 99, A custom exp at level 99, MZ custom exp at level 99, MS custom exp at level 99, ρ custom domain at level 99, r custom domain at level 99).
 Reserved Notation "'$|' m '&' n '|↘' r" (in custom judg at level 80, m custom domain at level 99, n custom domain at level 99, r custom domain at level 99).
-Reserved Notation "'⟦' σ '⟧s' p '↘' p'" (in custom judg at level 80, σ custom exp at level 99, p custom domain at level 99, p' custom domain at level 99).
+Reserved Notation "'⟦' σ '⟧s' ρ '↘' ρσ" (in custom judg at level 80, σ custom exp at level 99, ρ custom domain at level 99, ρσ custom domain at level 99).
 
 Generalizable All Variables.
 
 Inductive eval_exp : exp -> env -> domain -> Prop :=
 | eval_exp_typ :
-  `( {{ ⟦ Type@i ⟧ p ↘ 𝕌@i }} )
+  `( {{ ⟦ Type@i ⟧ ρ ↘ 𝕌@i }} )
 | eval_exp_var :
-  `( {{ ⟦ # x ⟧ p ↘ ~(p x) }} )
+  `( {{ ⟦ # x ⟧ ρ ↘ ~(ρ x) }} )
 | eval_exp_nat :
-  `( {{ ⟦ ℕ ⟧ p ↘ ℕ }} )
+  `( {{ ⟦ ℕ ⟧ ρ ↘ ℕ }} )
 | eval_exp_zero :
-  `( {{ ⟦ zero ⟧ p ↘ zero }} )
+  `( {{ ⟦ zero ⟧ ρ ↘ zero }} )
 | eval_exp_succ :
-  `( {{ ⟦ M ⟧ p ↘ m }} ->
-     {{ ⟦ succ M ⟧ p ↘ succ m }} )
+  `( {{ ⟦ M ⟧ ρ ↘ m }} ->
+     {{ ⟦ succ M ⟧ ρ ↘ succ m }} )
 | eval_exp_natrec :
-  `( {{ ⟦ M ⟧ p ↘ m }} ->
-     {{ rec m ⟦return A | zero -> MZ | succ -> MS end⟧ p ↘ r }} ->
-     {{ ⟦ rec M return A | zero -> MZ | succ -> MS end ⟧ p ↘ r }} )
+  `( {{ ⟦ M ⟧ ρ ↘ m }} ->
+     {{ rec m ⟦return A | zero -> MZ | succ -> MS end⟧ ρ ↘ r }} ->
+     {{ ⟦ rec M return A | zero -> MZ | succ -> MS end ⟧ ρ ↘ r }} )
 | eval_exp_pi :
-  `( {{ ⟦ A ⟧ p ↘ a }} ->
-     {{ ⟦ Π A B ⟧ p ↘ Π a p B }} )
+  `( {{ ⟦ A ⟧ ρ ↘ a }} ->
+     {{ ⟦ Π A B ⟧ ρ ↘ Π a ρ B }} )
 | eval_exp_fn :
-  `( {{ ⟦ λ A M ⟧ p ↘ λ p M }} )
+  `( {{ ⟦ λ A M ⟧ ρ ↘ λ ρ M }} )
 | eval_exp_app :
-  `( {{ ⟦ M ⟧ p ↘ m }} ->
-     {{ ⟦ N ⟧ p ↘ n }} ->
+  `( {{ ⟦ M ⟧ ρ ↘ m }} ->
+     {{ ⟦ N ⟧ ρ ↘ n }} ->
      {{ $| m & n |↘ r }} ->
-     {{ ⟦ M N ⟧ p ↘ r }} )
+     {{ ⟦ M N ⟧ ρ ↘ r }} )
 | eval_exp_sub :
-  `( {{ ⟦ σ ⟧s p ↘ p' }} ->
-     {{ ⟦ M ⟧ p' ↘ m }} ->
-     {{ ⟦ M[σ] ⟧ p ↘ m }} )
-where "'⟦' e '⟧' p '↘' r" := (eval_exp e p r) (in custom judg)
+  `( {{ ⟦ σ ⟧s ρ ↘ ρ' }} ->
+     {{ ⟦ M ⟧ ρ' ↘ m }} ->
+     {{ ⟦ M[σ] ⟧ ρ ↘ m }} )
+where "'⟦' e '⟧' ρ '↘' r" := (eval_exp e ρ r) (in custom judg)
 with eval_natrec : exp -> exp -> exp -> domain -> env -> domain -> Prop :=
 | eval_natrec_zero :
-  `( {{ ⟦ MZ ⟧ p ↘ mz }} ->
-     {{ rec zero ⟦return A | zero -> MZ | succ -> MS end⟧ p ↘ mz }} )
+  `( {{ ⟦ MZ ⟧ ρ ↘ mz }} ->
+     {{ rec zero ⟦return A | zero -> MZ | succ -> MS end⟧ ρ ↘ mz }} )
 | eval_natrec_succ :
-  `( {{ rec b ⟦return A | zero -> MZ | succ -> MS end⟧ p ↘ r }} ->
-     {{ ⟦ MS ⟧ p ↦ b ↦ r ↘ ms }} ->
-     {{ rec succ b ⟦return A | zero -> MZ | succ -> MS end⟧ p ↘ ms }} )
+  `( {{ rec b ⟦return A | zero -> MZ | succ -> MS end⟧ ρ ↘ r }} ->
+     {{ ⟦ MS ⟧ ρ ↦ b ↦ r ↘ ms }} ->
+     {{ rec succ b ⟦return A | zero -> MZ | succ -> MS end⟧ ρ ↘ ms }} )
 | eval_natrec_neut :
-  `( {{ ⟦ MZ ⟧ p ↘ mz }} ->
-     {{ ⟦ A ⟧ p ↦ ⇑ ℕ m ↘ a }} ->
-     {{ rec ⇑ ℕ m ⟦return A | zero -> MZ | succ -> MS end⟧ p ↘ ⇑ a (rec m under p return A | zero -> mz | succ -> MS end) }} )
-where "'rec' m '⟦return' A | 'zero' -> MZ | 'succ' -> MS 'end⟧' p '↘' r" := (eval_natrec A MZ MS m p r) (in custom judg)
+  `( {{ ⟦ MZ ⟧ ρ ↘ mz }} ->
+     {{ ⟦ A ⟧ ρ ↦ ⇑ ℕ m ↘ a }} ->
+     {{ rec ⇑ ℕ m ⟦return A | zero -> MZ | succ -> MS end⟧ ρ ↘ ⇑ a (rec m under ρ return A | zero -> mz | succ -> MS end) }} )
+where "'rec' m '⟦return' A | 'zero' -> MZ | 'succ' -> MS 'end⟧' ρ '↘' r" := (eval_natrec A MZ MS m ρ r) (in custom judg)
 with eval_app : domain -> domain -> domain -> Prop :=
 | eval_app_fn :
-  `( {{ ⟦ M ⟧ p ↦ n ↘ m }} ->
-     {{ $| λ p M & n |↘ m }} )
+  `( {{ ⟦ M ⟧ ρ ↦ n ↘ m }} ->
+     {{ $| λ ρ M & n |↘ m }} )
 | eval_app_neut :
-  `( {{ ⟦ B ⟧ p ↦ n ↘ b }} ->
-     {{ $| ⇑ (Π a p B) m & n |↘ ⇑ b (m (⇓ a n)) }} )
+  `( {{ ⟦ B ⟧ ρ ↦ n ↘ b }} ->
+     {{ $| ⇑ (Π a ρ B) m & n |↘ ⇑ b (m (⇓ a n)) }} )
 where "'$|' m '&' n '|↘' r" := (eval_app m n r) (in custom judg)
 with eval_sub : sub -> env -> env -> Prop :=
 | eval_sub_id :
-  `( {{ ⟦ Id ⟧s p ↘ p }} )
+  `( {{ ⟦ Id ⟧s ρ ↘ ρ }} )
 | eval_sub_weaken :
-  `( {{ ⟦ Wk ⟧s p ↘ p↯ }} )
+  `( {{ ⟦ Wk ⟧s ρ ↘ ρ ↯ }} )
 | eval_sub_extend :
-  `( {{ ⟦ σ ⟧s p ↘ p' }} ->
-     {{ ⟦ M ⟧ p ↘ m }} ->
-     {{ ⟦ σ ,, M ⟧s p ↘ p' ↦ m }} )
+  `( {{ ⟦ σ ⟧s ρ ↘ ρσ }} ->
+     {{ ⟦ M ⟧ ρ ↘ m }} ->
+     {{ ⟦ σ ,, M ⟧s ρ ↘ ρσ ↦ m }} )
 | eval_sub_compose :
-  `( {{ ⟦ τ ⟧s p ↘ p' }} ->
-     {{ ⟦ σ ⟧s p' ↘ p'' }} ->
-     {{ ⟦ σ ∘ τ ⟧s p ↘ p'' }} )
-where "'⟦' σ '⟧s' p '↘' p'" := (eval_sub σ p p') (in custom judg)
+  `( {{ ⟦ τ ⟧s ρ ↘ ρτ }} ->
+     {{ ⟦ σ ⟧s ρτ ↘ ρτσ }} ->
+     {{ ⟦ σ ∘ τ ⟧s ρ ↘ ρτσ }} )
+where "'⟦' σ '⟧s' ρ '↘' ρσ" := (eval_sub σ ρ ρσ) (in custom judg)
 .
 
 Scheme eval_exp_mut_ind := Induction for eval_exp Sort Prop
 with eval_natrec_mut_ind := Induction for eval_natrec Sort Prop
 with eval_app_mut_ind := Induction for eval_app Sort Prop
 with eval_sub_mut_ind := Induction for eval_sub Sort Prop.
+Combined Scheme eval_mut_ind from
+  eval_exp_mut_ind,
+  eval_natrec_mut_ind,
+  eval_app_mut_ind,
+  eval_sub_mut_ind.
 
 #[export]
 Hint Constructors eval_exp eval_natrec eval_app eval_sub : mcltt.
