theories/Core/Completeness/LogicalRelation/Lemmas.v
@@ -3,23 +3,23 @@ From Mcltt Require Import Base LibTactics.
 From Mcltt.Core.Completeness Require Import LogicalRelation.Definitions LogicalRelation.Tactics.
 Import Domain_Notations.
 
-Add Parametric Morphism M p M' p' : (rel_exp M p M' p')
+Add Parametric Morphism M ρ M' ρ' : (rel_exp M ρ M' ρ')
     with signature (@relation_equivalence domain) ==> iff as rel_exp_morphism.
 Proof.
   intros R R' HRR'.
   split; intros []; econstructor; intuition.
 Qed.
 
-Add Parametric Morphism σ p σ' p' : (rel_sub σ p σ' p')
+Add Parametric Morphism σ ρ σ' ρ' : (rel_sub σ ρ σ' ρ')
     with signature (@relation_equivalence env) ==> iff as rel_sub_morphism.
 Proof.
   intros R R' HRR'.
   split; intros []; econstructor; intuition.
 Qed.
 
-Lemma rel_exp_implies_rel_typ : forall {i A p A' p'},
-    rel_exp A p A' p' (per_univ i) ->
-    exists R, rel_typ i A p A' p' R.
+Lemma rel_exp_implies_rel_typ : forall {i A ρ A' ρ'},
+    rel_exp A ρ A' ρ' (per_univ i) ->
+    exists R, rel_typ i A ρ A' ρ' R.
 Proof.
   intros.
   destruct_by_head rel_exp.
@@ -30,9 +30,9 @@ Qed.
 #[export]
 Hint Resolve rel_exp_implies_rel_typ : mcltt.
 
-Lemma rel_typ_implies_rel_exp : forall {i A p A' p' R},
-    rel_typ i A p A' p' R ->
-    rel_exp A p A' p' (per_univ i).
+Lemma rel_typ_implies_rel_exp : forall {i A ρ A' ρ' R},
+    rel_typ i A ρ A' ρ' R ->
+    rel_exp A ρ A' ρ' (per_univ i).
 Proof.
   intros.
   destruct_by_head rel_typ.
