theories/Core/Completeness/UniverseCases.v
@@ -7,8 +7,8 @@ Import Domain_Notations.
 Lemma rel_exp_of_typ_inversion : forall {Γ A A' i},
     {{ Γ ⊨ A ≈ A' : Type@i }} ->
     exists env_rel (_ : {{ EF Γ ≈ Γ ∈ per_ctx_env ↘ env_rel }}),
-    forall p p' (equiv_p_p' : {{ Dom p ≈ p' ∈ env_rel }}),
-      rel_exp A p A' p' (per_univ i).
+    forall ρ ρ' (equiv_ρ_ρ' : {{ Dom ρ ≈ ρ' ∈ env_rel }}),
+      rel_exp A ρ A' ρ' (per_univ i).
 Proof.
   intros * [env_relΓ].
   destruct_conjs.
@@ -23,8 +23,8 @@ Qed.
 
 Lemma rel_exp_of_typ : forall {Γ A A' i},
     (exists env_rel (_ : {{ EF Γ ≈ Γ ∈ per_ctx_env ↘ env_rel }}),
-      forall p p' (equiv_p_p' : {{ Dom p ≈ p' ∈ env_rel }}),
-        rel_exp A p A' p' (per_univ i)) ->
+      forall ρ ρ' (equiv_ρ_ρ' : {{ Dom ρ ≈ ρ' ∈ env_rel }}),
+        rel_exp A ρ A' ρ' (per_univ i)) ->
     {{ Γ ⊨ A ≈ A' : Type@i }}.
 Proof.
   intros * [env_relΓ].
