theories/Core/Semantic/Evaluation/Lemmas.v
@@ -3,58 +3,62 @@ From Mcltt Require Import Base LibTactics Evaluation.Definitions.
 Import Domain_Notations.
 
 Section functional_eval.
-  Let functional_eval_exp_prop M p m1 (_ : {{ ⟦ M ⟧ p ↘ m1 }}) : Prop := forall m2 (Heval2: {{ ⟦ M ⟧ p ↘ m2 }}), m1 = m2.
-  Let functional_eval_natrec_prop A MZ MS m p r1 (_ : {{ rec m ⟦return A | zero -> MZ | succ -> MS end⟧ p ↘ r1 }}) : Prop := forall r2 (Heval2 : {{ rec m ⟦return A | zero -> MZ | succ -> MS end⟧ p ↘ r2 }}), r1 = r2.
-  Let functional_eval_app_prop m n r1 (_ : {{ $| m & n |↘ r1 }}) : Prop := forall r2 (Heval2 : {{ $| m & n |↘ r2 }}), r1 = r2.
-  Let functional_eval_sub_prop σ p p1 (_ : {{ ⟦ σ ⟧s p ↘ p1 }}) : Prop := forall p2 (Heval2 : {{ ⟦ σ ⟧s p ↘ p2 }}), p1 = p2.
-
-  #[local]
-  Ltac unfold_functional_eval :=
-    unfold functional_eval_exp_prop, functional_eval_natrec_prop, functional_eval_app_prop, functional_eval_sub_prop in *;
-    clear functional_eval_exp_prop functional_eval_natrec_prop functional_eval_app_prop functional_eval_sub_prop.
-
-  Lemma functional_eval_exp : forall M p m1 (Heval1 : {{ ⟦ M ⟧ p ↘ m1 }}), functional_eval_exp_prop M p m1 Heval1.
+  Lemma functional_eval :
+    (forall M ρ m1,
+        {{ ⟦ M ⟧ ρ ↘ m1 }} ->
+        forall m2,
+          {{ ⟦ M ⟧ ρ ↘ m2 }} ->
+          m1 = m2) /\
+      (forall A MZ MS m ρ r1,
+          {{ rec m ⟦return A | zero -> MZ | succ -> MS end⟧ ρ ↘ r1 }} ->
+          forall r2,
+            {{ rec m ⟦return A | zero -> MZ | succ -> MS end⟧ ρ ↘ r2 }} ->
+            r1 = r2) /\
+      (forall m n r1,
+          {{ $| m & n |↘ r1 }} ->
+          forall r2,
+            {{ $| m & n |↘ r2 }} ->
+            r1 = r2) /\
+      (forall σ ρ ρσ1,
+          {{ ⟦ σ ⟧s ρ ↘ ρσ1 }} ->
+          forall ρσ2,
+            {{ ⟦ σ ⟧s ρ ↘ ρσ2 }} ->
+            ρσ1 = ρσ2).
   Proof with ((on_all_hyp: fun H => erewrite H in *; eauto); solve [eauto]) using.
-    induction Heval1
-      using eval_exp_mut_ind
-      with (P0 := functional_eval_natrec_prop)
-           (P1 := functional_eval_app_prop)
-           (P2 := functional_eval_sub_prop);
-      unfold_functional_eval;
-      inversion_clear 1; do 2 f_equal...
+    apply eval_mut_ind; intros;
+      progressive_inversion; do 2 f_equal; try reflexivity...
   Qed.
 
-  Lemma functional_eval_natrec : forall A MZ MS m p r1 (Heval1 : {{ rec m ⟦return A | zero -> MZ | succ -> MS end⟧ p ↘ r1 }}), functional_eval_natrec_prop A MZ MS m p r1 Heval1.
-  Proof with ((on_all_hyp: fun H => erewrite H in *; eauto); solve [eauto]) using.
-    induction Heval1
-      using eval_natrec_mut_ind
-      with (P := functional_eval_exp_prop)
-           (P1 := functional_eval_app_prop)
-           (P2 := functional_eval_sub_prop);
-      unfold_functional_eval;
-      inversion_clear 1; do 2 f_equal...
+  Corollary functional_eval_exp : forall M ρ m1 m2,
+      {{ ⟦ M ⟧ ρ ↘ m1 }} ->
+      {{ ⟦ M ⟧ ρ ↘ m2 }} ->
+      m1 = m2.
+  Proof.
+    pose proof functional_eval; firstorder.
   Qed.
 
-  Lemma functional_eval_app : forall m n r1 (Heval1 : {{ $| m & n |↘ r1 }}), functional_eval_app_prop m n r1 Heval1.
-  Proof with ((on_all_hyp: fun H => erewrite H in *; eauto); solve [eauto]) using.
-    induction Heval1
-      using eval_app_mut_ind
-      with (P := functional_eval_exp_prop)
-           (P0 := functional_eval_natrec_prop)
-           (P2 := functional_eval_sub_prop);
-      unfold_functional_eval;
-      inversion_clear 1; do 2 f_equal...
+  Corollary functional_eval_natrec : forall A MZ MS m ρ r1 r2,
+      {{ rec m ⟦return A | zero -> MZ | succ -> MS end⟧ ρ ↘ r1 }} ->
+      {{ rec m ⟦return A | zero -> MZ | succ -> MS end⟧ ρ ↘ r2 }} ->
+      r1 = r2.
+  Proof.
+    pose proof functional_eval; intuition.
   Qed.
 
-  Lemma functional_eval_sub : forall σ p p1 (Heval1 : {{ ⟦ σ ⟧s p ↘ p1 }}), functional_eval_sub_prop σ p p1 Heval1.
-  Proof with ((on_all_hyp: fun H => erewrite H in *; eauto); solve [eauto]) using.
-    induction Heval1
-      using eval_sub_mut_ind
-      with (P := functional_eval_exp_prop)
-           (P0 := functional_eval_natrec_prop)
-           (P1 := functional_eval_app_prop);
-      unfold_functional_eval;
-      inversion_clear 1; do 2 f_equal...
+  Corollary functional_eval_app : forall m n r1 r2,
+      {{ $| m & n |↘ r1 }} ->
+      {{ $| m & n |↘ r2 }} ->
+      r1 = r2.
+  Proof.
+    pose proof functional_eval; intuition.
+  Qed.
+
+  Corollary functional_eval_sub : forall σ ρ ρσ1 ρσ2,
+      {{ ⟦ σ ⟧s ρ ↘ ρσ1 }} ->
+      {{ ⟦ σ ⟧s ρ ↘ ρσ2 }} ->
+      ρσ1 = ρσ2.
+  Proof.
+    pose proof functional_eval; firstorder.
   Qed.
 End functional_eval.
 
@@ -64,13 +68,13 @@ Hint Resolve functional_eval_exp functional_eval_natrec functional_eval_app func
 Ltac functional_eval_rewrite_clear1 :=
   let tactic_error o1 o2 := fail 3 "functional_eval equality between" o1 "and" o2 "cannot be solved by mauto" in
   match goal with
-  | H1 : {{ ⟦ ~?M ⟧ ~?p ↘ ~?m1 }}, H2 : {{ ⟦ ~?M ⟧ ~?p ↘ ~?m2 }} |- _ =>
+  | H1 : {{ ⟦ ~?M ⟧ ~?ρ ↘ ~?m1 }}, H2 : {{ ⟦ ~?M ⟧ ~?ρ ↘ ~?m2 }} |- _ =>
       clean replace m2 with m1 by first [solve [mauto 2] | tactic_error m2 m1]; clear H2
   | H1 : {{ $| ~?m & ~?n |↘ ~?r1 }}, H2 : {{ $| ~?m & ~?n |↘ ~?r2 }} |- _ =>
       clean replace r2 with r1 by first [solve [mauto 2] | tactic_error r2 r1]; clear H2
-  | H1 : {{ rec ~?m ⟦return ~?A | zero -> ~?MZ | succ -> ~?MS end⟧ ~?p ↘ ~?r1 }}, H2 : {{ rec ~?m ⟦return ~?A | zero -> ~?MZ | succ -> ~?MS end⟧ ~?p ↘ ~?r2 }} |- _ =>
+  | H1 : {{ rec ~?m ⟦return ~?A | zero -> ~?MZ | succ -> ~?MS end⟧ ~?ρ ↘ ~?r1 }}, H2 : {{ rec ~?m ⟦return ~?A | zero -> ~?MZ | succ -> ~?MS end⟧ ~?ρ ↘ ~?r2 }} |- _ =>
       clean replace r2 with r1 by first [solve [mauto 2] | tactic_error r2 r1]; clear H2
-  | H1 : {{ ⟦ ~?σ ⟧s ~?p ↘ ~?p1 }}, H2 : {{ ⟦ ~?σ ⟧s ~?p ↘ ~?p2 }} |- _ =>
-      clean replace p2 with p1 by first [solve [mauto 2] | tactic_error p2 p1]; clear H2
+  | H1 : {{ ⟦ ~?σ ⟧s ~?ρ ↘ ~?ρσ1 }}, H2 : {{ ⟦ ~?σ ⟧s ~?ρ ↘ ~?ρσ2 }} |- _ =>
+      clean replace ρσ2 with ρσ1 by first [solve [mauto 2] | tactic_error ρσ2 ρσ1]; clear H2
   end.
 Ltac functional_eval_rewrite_clear := repeat functional_eval_rewrite_clear1.
