theories/Core/Semantic/Evaluation/Tactics.v
@@ -4,7 +4,9 @@ Import Domain_Notations.
 Ltac simplify_evals :=
   functional_eval_rewrite_clear;
   clear_dups;
-  repeat (match_by_head eval_exp ltac:(fun H => directed inversion H; subst; clear H)
-          || match_by_head eval_sub ltac:(fun H => directed inversion H; subst; clear H));
+  repeat (match_by_head eval_exp ltac:(fun H => directed dependent destruction H)
+          || match_by_head eval_app ltac:(fun H => directed dependent destruction H)
+          || match_by_head eval_natrec ltac:(fun H => directed dependent destruction H)
+          || match_by_head eval_sub ltac:(fun H => directed dependent destruction H));
   functional_eval_rewrite_clear;
   clear_dups.
