theories/Core/Soundness/LogicalRelation/CoreLemmas.v
@@ -6,8 +6,8 @@ From Mcltt.Core.Soundness Require Import LogicalRelation.Definitions LogicalRela
 From Mcltt.Core.Soundness Require Export Weakening.Lemmas.
 Import Domain_Notations.
 
-Lemma glu_nat_per_nat : forall Γ m a,
-    glu_nat Γ m a ->
+Lemma glu_nat_per_nat : forall Γ M a,
+    glu_nat Γ M a ->
     {{ Dom a ≈ a ∈ per_nat }}.
 Proof.
   induction 1; mauto.
@@ -16,19 +16,19 @@ Qed.
 #[local]
 Hint Resolve glu_nat_per_nat : mcltt.
 
-Lemma glu_nat_escape : forall Γ m a,
-    glu_nat Γ m a ->
+Lemma glu_nat_escape : forall Γ M a,
+    glu_nat Γ M a ->
     {{ ⊢ Γ }} ->
-    {{ Γ ⊢ m : ℕ }}.
+    {{ Γ ⊢ M : ℕ }}.
 Proof.
   induction 1; intros;
     try match goal with
     | H : _ |- _ => solve [gen_presup H; mauto]
     end.
   assert {{ Γ ⊢w Id : Γ }} by mauto.
-  match_by_head (per_bot c c) ltac:(fun H => specialize (H (length Γ)) as [L []]).
+  match_by_head (per_bot m m) ltac:(fun H => specialize (H (length Γ)) as [M' []]).
   clear_dups.
-  assert {{ Γ ⊢ m[Id] ≈ L : ℕ }} by mauto.
+  assert {{ Γ ⊢ M[Id] ≈ M' : ℕ }} by mauto.
   gen_presups.
   mauto.
 Qed.
@@ -36,10 +36,10 @@ Qed.
 #[export]
 Hint Resolve glu_nat_escape : mcltt.
 
-Lemma glu_nat_resp_ctx_eq : forall Γ m a Δ,
-    glu_nat Γ m a ->
+Lemma glu_nat_resp_ctx_eq : forall Γ M a Δ,
+    glu_nat Γ M a ->
     {{ ⊢ Γ ≈ Δ }} ->
-    glu_nat Δ m a.
+    glu_nat Δ M a.
 Proof.
   induction 1; intros; mauto.
 Qed.
@@ -53,16 +53,16 @@ Proof.
   split; mauto using glu_nat_resp_ctx_eq.
 Qed.
 
-Lemma glu_nat_resp_exp_eq : forall Γ m a,
-    glu_nat Γ m a ->
-    forall m',
-    {{ Γ ⊢ m ≈ m' : ℕ }} ->
-    glu_nat Γ m' a.
+Lemma glu_nat_resp_exp_eq : forall Γ M a,
+    glu_nat Γ M a ->
+    forall M',
+    {{ Γ ⊢ M ≈ M' : ℕ }} ->
+    glu_nat Γ M' a.
 Proof.
   induction 1; intros; mauto.
   econstructor; trivial.
   intros.
-  transitivity {{{ m[σ] }}}; mauto.
+  transitivity {{{ M[σ] }}}; mauto.
 Qed.
 
 #[local]
@@ -74,18 +74,18 @@ Proof.
   split; mauto using glu_nat_resp_exp_eq.
 Qed.
 
-Lemma glu_nat_readback : forall Γ m a,
-    glu_nat Γ m a ->
-    forall Δ σ b,
+Lemma glu_nat_readback : forall Γ M a,
+    glu_nat Γ M a ->
+    forall Δ σ M',
       {{ Δ ⊢w σ : Γ }} ->
-      {{ Rnf ⇓ ℕ a in length Δ ↘ b }} ->
-      {{ Δ ⊢ m [ σ ] ≈ b : ℕ }}.
+      {{ Rnf ⇓ ℕ a in length Δ ↘ M' }} ->
+      {{ Δ ⊢ M[σ] ≈ M' : ℕ }}.
 Proof.
   induction 1; intros; progressive_inversion; gen_presups.
   - transitivity {{{ zero[σ] }}}; mauto.
-  - assert {{ Δ ⊢ m'[σ] ≈ M : ℕ }} by mauto.
-    transitivity {{{ (succ m')[σ] }}}; mauto 3.
-    transitivity {{{ succ m'[σ] }}}; mauto 4.
+  - assert {{ Δ ⊢ M'[σ] ≈ M0 : ℕ }} by mauto.
+    transitivity {{{ (succ M')[σ] }}}; mauto 3.
+    transitivity {{{ succ M'[σ] }}}; mauto 4.
   - mauto.
 Qed.
 
@@ -97,23 +97,23 @@ Ltac simpl_glu_rel :=
   destruct_all;
   gen_presups.
 
-Lemma glu_univ_elem_univ_lvl : forall i P El A,
-    {{ DG A ∈ glu_univ_elem i ↘ P ↘ El }} ->
-    forall Γ T,
-      {{ Γ ⊢ T ® P }} ->
-      {{ Γ ⊢ T : Type@i }}.
+Lemma glu_univ_elem_univ_lvl : forall i P El a,
+    {{ DG a ∈ glu_univ_elem i ↘ P ↘ El }} ->
+    forall Γ A,
+      {{ Γ ⊢ A ® P }} ->
+      {{ Γ ⊢ A : Type@i }}.
 Proof.
   simpl.
   induction 1 using glu_univ_elem_ind; intros;
     simpl_glu_rel; trivial.
 Qed.
 
-Lemma glu_univ_elem_typ_resp_exp_eq : forall i P El A,
-    {{ DG A ∈ glu_univ_elem i ↘ P ↘ El }} ->
-    forall Γ T T',
-      {{ Γ ⊢ T ® P }} ->
-      {{ Γ ⊢ T ≈ T' : Type@i }} ->
-      {{ Γ ⊢ T' ® P }}.
+Lemma glu_univ_elem_typ_resp_exp_eq : forall i P El a,
+    {{ DG a ∈ glu_univ_elem i ↘ P ↘ El }} ->
+    forall Γ A A',
+      {{ Γ ⊢ A ® P }} ->
+      {{ Γ ⊢ A ≈ A' : Type@i }} ->
+      {{ Γ ⊢ A' ® P }}.
 Proof.
   simpl.
   induction 1 using glu_univ_elem_ind; intros;
@@ -121,29 +121,31 @@ Proof.
 
   split; [trivial |].
   intros.
-  assert {{ Δ ⊢ T[σ] ≈ V : Type@i }}; mauto.
+  transitivity {{{ A[σ] }}}; mauto 4.
 Qed.
 
-Add Parametric Morphism i P El A (H : glu_univ_elem i P El A) Γ : (P Γ)
-    with signature wf_exp_eq Γ {{{Type@i}}} ==> iff as glu_univ_elem_typ_morphism_iff1.
+Add Parametric Morphism i P El a (H : glu_univ_elem i P El a) Γ : (P Γ)
+    with signature wf_exp_eq Γ {{{ Type@i }}} ==> iff as glu_univ_elem_typ_morphism_iff1.
 Proof.
   split; intros; eapply glu_univ_elem_typ_resp_exp_eq; mauto 2.
 Qed.
 
-Lemma glu_univ_elem_trm_resp_typ_exp_eq : forall i P El A,
-    {{ DG A ∈ glu_univ_elem i ↘ P ↘ El }} ->
-    forall Γ t T a T',
-      {{ Γ ⊢ t : T ® a ∈ El }} ->
-      {{ Γ ⊢ T ≈ T' : Type@i }} ->
-      {{ Γ ⊢ t : T' ® a ∈ El }}.
+Lemma glu_univ_elem_trm_resp_typ_exp_eq : forall i P El a,
+    {{ DG a ∈ glu_univ_elem i ↘ P ↘ El }} ->
+    forall Γ M A m A',
+      {{ Γ ⊢ M : A ® m ∈ El }} ->
+      {{ Γ ⊢ A ≈ A' : Type@i }} ->
+      {{ Γ ⊢ M : A' ® m ∈ El }}.
 Proof.
   simpl.
   induction 1 using glu_univ_elem_ind; intros;
     simpl_glu_rel; repeat split; intros; mauto 3;
-    [firstorder | | assert {{ Δ ⊢ M[σ] ≈ V : Type@i }} by mauto 3 |]; mauto.
+    [firstorder | | transitivity {{{ A[σ] }}}; mauto 4 | assert {{ Δ ⊢ A[σ] ≈ A'[σ] : Type@i }}; mauto 3].
+
+  econstructor; mauto 3.
 Qed.
 
-Add Parametric Morphism i P El A (H : glu_univ_elem i P El A) Γ : (El Γ)
+Add Parametric Morphism i P El a (H : glu_univ_elem i P El a) Γ : (El Γ)
     with signature wf_exp_eq Γ {{{Type@i}}} ==> eq ==> eq ==> iff as glu_univ_elem_trm_morphism_iff1.
 Proof.
   split; intros;
@@ -151,12 +153,12 @@ Proof.
     mauto 2.
 Qed.
 
-Lemma glu_univ_elem_typ_resp_ctx_eq : forall i P El A,
-    {{ DG A ∈ glu_univ_elem i ↘ P ↘ El }} ->
-    forall Γ T Δ,
-      {{ Γ ⊢ T ® P }} ->
+Lemma glu_univ_elem_typ_resp_ctx_eq : forall i P El a,
+    {{ DG a ∈ glu_univ_elem i ↘ P ↘ El }} ->
+    forall Γ A Δ,
+      {{ Γ ⊢ A ® P }} ->
       {{ ⊢ Γ ≈ Δ }} ->
-      {{ Δ ⊢ T ® P }}.
+      {{ Δ ⊢ A ® P }}.
 Proof.
   simpl.
   induction 1 using glu_univ_elem_ind; intros;
@@ -164,7 +166,7 @@ Proof.
     econstructor; mauto 4.
 Qed.
 
-Add Parametric Morphism i P El A (H : glu_univ_elem i P El A) : P
+Add Parametric Morphism i P El a (H : glu_univ_elem i P El a) : P
     with signature wf_ctx_eq ==> eq ==> iff as glu_univ_elem_typ_morphism_iff2.
 Proof.
   intros. split; intros;
@@ -172,12 +174,12 @@ Proof.
     mauto 2.
 Qed.
 
-Lemma glu_univ_elem_trm_resp_ctx_eq : forall i P El A,
-    {{ DG A ∈ glu_univ_elem i ↘ P ↘ El }} ->
-    forall Γ T M m Δ,
-      {{ Γ ⊢ M : T ® m ∈ El }} ->
+Lemma glu_univ_elem_trm_resp_ctx_eq : forall i P El a,
+    {{ DG a ∈ glu_univ_elem i ↘ P ↘ El }} ->
+    forall Γ A M m Δ,
+      {{ Γ ⊢ M : A ® m ∈ El }} ->
       {{ ⊢ Γ ≈ Δ }} ->
-      {{ Δ ⊢ M : T ® m ∈ El }}.
+      {{ Δ ⊢ M : A ® m ∈ El }}.
 Proof.
   simpl.
   induction 1 using glu_univ_elem_ind; intros;
@@ -191,7 +193,7 @@ Proof.
   - split; mauto 4.
 Qed.
 
-Add Parametric Morphism i P El A (H : glu_univ_elem i P El A) : El
+Add Parametric Morphism i P El a (H : glu_univ_elem i P El a) : El
     with signature wf_ctx_eq ==> eq ==> eq ==> eq ==> iff as glu_univ_elem_trm_morphism_iff2.
 Proof.
   intros. split; intros;
@@ -199,30 +201,31 @@ Proof.
     mauto 2.
 Qed.
 
-Lemma glu_nat_resp_wk' : forall Γ m a,
-    glu_nat Γ m a ->
+Lemma glu_nat_resp_wk' : forall Γ M a,
+    glu_nat Γ M a ->
     forall Δ σ,
-      {{ Γ ⊢ m : ℕ }} ->
+      {{ Γ ⊢ M : ℕ }} ->
       {{ Δ ⊢w σ : Γ }} ->
-      glu_nat Δ {{{ m[σ] }}} a.
+      glu_nat Δ {{{ M[σ] }}} a.
 Proof.
   induction 1; intros; gen_presups.
   - econstructor.
     transitivity {{{ zero[σ] }}}; mauto.
   - econstructor; [ |mauto].
-    transitivity {{{ (succ m')[σ] }}}; mauto 4.
+    transitivity {{{ (succ M')[σ] }}}; mauto 4.
   - econstructor; trivial.
-    intros. gen_presups.
-    assert {{ Δ0 ⊢w σ ∘ σ0 : Γ }} by mauto.
-    assert {{ Δ0 ⊢ m[σ ∘ σ0] ≈ v : ℕ }} by mauto 4.
-    transitivity {{{ m[σ ∘ σ0] }}}; mauto 4.
+    intros Δ' τ M' **.
+    gen_presups.
+    assert {{ Δ' ⊢w σ∘τ : Γ }} by mauto.
+    assert {{ Δ' ⊢ M[σ∘τ] ≈ M' : ℕ }} by mauto 4.
+    transitivity {{{ M[σ∘τ] }}}; mauto 4.
 Qed.
 
-Lemma glu_nat_resp_wk : forall Γ m a,
-    glu_nat Γ m a ->
+Lemma glu_nat_resp_wk : forall Γ M a,
+    glu_nat Γ M a ->
     forall Δ σ,
       {{ Δ ⊢w σ : Γ }} ->
-      glu_nat Δ {{{ m[σ] }}} a.
+      glu_nat Δ {{{ M[σ] }}} a.
 Proof.
   mauto using glu_nat_resp_wk'.
 Qed.
@@ -230,20 +233,20 @@ Qed.
 #[export]
 Hint Resolve glu_nat_resp_wk : mcltt.
 
-Lemma glu_univ_elem_trm_escape : forall i P El A,
-    {{ DG A ∈ glu_univ_elem i ↘ P ↘ El }} ->
-    forall Γ t T a,
-      {{ Γ ⊢ t : T ® a ∈ El }} ->
-      {{ Γ ⊢ t : T }}.
+Lemma glu_univ_elem_trm_escape : forall i P El a,
+    {{ DG a ∈ glu_univ_elem i ↘ P ↘ El }} ->
+    forall Γ M A m,
+      {{ Γ ⊢ M : A ® m ∈ El }} ->
+      {{ Γ ⊢ M : A }}.
 Proof.
   simpl.
   induction 1 using glu_univ_elem_ind; intros;
     simpl_glu_rel; mauto 4.
 Qed.
 
-Lemma glu_univ_elem_per_univ : forall i P El A,
-    {{ DG A ∈ glu_univ_elem i ↘ P ↘ El }} ->
-    {{ Dom A ≈ A ∈ per_univ i }}.
+Lemma glu_univ_elem_per_univ : forall i P El a,
+    {{ DG a ∈ glu_univ_elem i ↘ P ↘ El }} ->
+    {{ Dom a ≈ a ∈ per_univ i }}.
 Proof.
   simpl.
   induction 1 using glu_univ_elem_ind; intros; eexists;
@@ -258,18 +261,18 @@ Qed.
 #[export]
 Hint Resolve glu_univ_elem_per_univ : mcltt.
 
-Lemma glu_univ_elem_per_elem : forall i P El A,
-    {{ DG A ∈ glu_univ_elem i ↘ P ↘ El }} ->
-    forall Γ t T a R,
-      {{ Γ ⊢ t : T ® a ∈ El }} ->
-      {{ DF A ≈ A ∈ per_univ_elem i ↘ R }} ->
-      {{ Dom a ≈ a ∈ R }}.
+Lemma glu_univ_elem_per_elem : forall i P El a,
+    {{ DG a ∈ glu_univ_elem i ↘ P ↘ El }} ->
+    forall Γ M A m R,
+      {{ Γ ⊢ M : A ® m ∈ El }} ->
+      {{ DF a ≈ a ∈ per_univ_elem i ↘ R }} ->
+      {{ Dom m ≈ m ∈ R }}.
 Proof.
   simpl.
   induction 1 using glu_univ_elem_ind; intros;
     try do 2 match_by_head1 per_univ_elem invert_per_univ_elem;
     simpl_glu_rel;
-    try fold (per_univ j a a);
+    try fold (per_univ j m m);
     mauto 4.
 
   intros.
@@ -281,11 +284,11 @@ Proof.
   econstructor; firstorder eauto.
 Qed.
 
-Lemma glu_univ_elem_trm_typ : forall i P El A,
-    {{ DG A ∈ glu_univ_elem i ↘ P ↘ El }} ->
-    forall Γ t T a,
-      {{ Γ ⊢ t : T ® a ∈ El }} ->
-      {{ Γ ⊢ T ® P }}.
+Lemma glu_univ_elem_trm_typ : forall i P El a,
+    {{ DG a ∈ glu_univ_elem i ↘ P ↘ El }} ->
+    forall Γ M A m,
+      {{ Γ ⊢ M : A ® m ∈ El }} ->
+      {{ Γ ⊢ A ® P }}.
 Proof.
   simpl.
   induction 1 using glu_univ_elem_ind; intros;
@@ -294,26 +297,26 @@ Proof.
 
   econstructor; eauto.
   match_by_head per_univ_elem ltac:(fun H => directed invert_per_univ_elem H).
-  intros.
+  intros ? ? N n ? ? equiv_n.
   destruct_rel_mod_eval.
-  edestruct H12 as [? []]; eauto.
+  enough (exists mn : domain, {{ $| m & n |↘ mn }} /\  {{ Δ ⊢ M[σ] N : OT[σ,,N] ® mn ∈ OEl n equiv_n }}) as [? []]; eauto 3.
 Qed.
 
-Lemma glu_univ_elem_trm_univ_lvl : forall i P El A,
-    {{ DG A ∈ glu_univ_elem i ↘ P ↘ El }} ->
-    forall Γ t T a,
-      {{ Γ ⊢ t : T ® a ∈ El }} ->
-      {{ Γ ⊢ T : Type@i }}.
+Lemma glu_univ_elem_trm_univ_lvl : forall i P El a,
+    {{ DG a ∈ glu_univ_elem i ↘ P ↘ El }} ->
+    forall Γ M A m,
+      {{ Γ ⊢ M : A ® m ∈ El }} ->
+      {{ Γ ⊢ A : Type@i }}.
 Proof.
   intros. eapply glu_univ_elem_univ_lvl; [| eapply glu_univ_elem_trm_typ]; eassumption.
 Qed.
 
-Lemma glu_univ_elem_trm_resp_exp_eq : forall i P El A,
-    {{ DG A ∈ glu_univ_elem i ↘ P ↘ El }} ->
-    forall Γ t T a t',
-      {{ Γ ⊢ t : T ® a ∈ El }} ->
-      {{ Γ ⊢ t ≈ t' : T }} ->
-      {{ Γ ⊢ t' : T ® a ∈ El }}.
+Lemma glu_univ_elem_trm_resp_exp_eq : forall i P El a,
+    {{ DG a ∈ glu_univ_elem i ↘ P ↘ El }} ->
+    forall Γ A M m M',
+      {{ Γ ⊢ M : A ® m ∈ El }} ->
+      {{ Γ ⊢ M ≈ M' : A }} ->
+      {{ Γ ⊢ M' : A ® m ∈ El }}.
 Proof.
   simpl.
   induction 1 using glu_univ_elem_ind; intros;
@@ -324,26 +327,25 @@ Proof.
     eapply glu_univ_elem_typ_resp_exp_eq; mauto.
 
   - econstructor; eauto.
-    invert_per_univ_elem H3.
+    match_by_head per_univ_elem ltac:(fun H => directed invert_per_univ_elem H).
     intros.
     destruct_rel_mod_eval.
-    assert {{ Δ ⊢ m' : IT [σ]}} by eauto using glu_univ_elem_trm_escape.
-    edestruct H13 as [? []]; eauto.
+    assert {{ Δ ⊢ N : IT[σ]}} by eauto using glu_univ_elem_trm_escape.
+    assert (exists mn : domain, {{ $| m & n |↘ mn }} /\  {{ Δ ⊢ M[σ] N : OT[σ,,N] ® mn ∈ OEl n equiv_n }}) as [? []] by intuition.
     eexists; split; eauto.
-    enough {{ Δ ⊢ m[σ] m' ≈ t'[σ] m' : OT[σ,,m'] }} by eauto.
-    assert {{ Γ ⊢ m ≈ t' : Π IT OT }} as Hty by mauto.
+    enough {{ Δ ⊢ M[σ] N ≈ M'[σ] N : OT[σ,,N] }} by eauto.
+    assert {{ Γ ⊢ M ≈ M' : Π IT OT }} as Hty by mauto.
     eassert {{ Δ ⊢ IT[σ] : Type@_ }} by mauto 3.
     eapply wf_exp_eq_sub_cong with (Γ := Δ) in Hty; [| eapply sub_eq_refl; mauto 3].
     autorewrite with mcltt in Hty.
-    eapply wf_exp_eq_app_cong with (N := m') (N' := m') in Hty; try pi_univ_level_tac; [|mauto 2].
+    eapply wf_exp_eq_app_cong with (N := N) (N' := N) in Hty; try pi_univ_level_tac; [|mauto 2].
     autorewrite with mcltt in Hty.
     eassumption.
   - intros.
-    assert {{ Δ ⊢ m[σ] ≈ t'[σ] : M[σ] }} by mauto 4.
-    mauto 4.
+    enough {{ Δ ⊢ M[σ] ≈ M'[σ] : A[σ] }}; mauto 4.
 Qed.
 
-Add Parametric Morphism i P El A (H : glu_univ_elem i P El A) Γ T : (El Γ T)
+Add Parametric Morphism i P El a (H : glu_univ_elem i P El a) Γ T : (El Γ T)
     with signature wf_exp_eq Γ T ==> eq ==> iff as glu_univ_elem_trm_morphism_iff3.
 Proof.
   split; intros;
@@ -412,7 +414,7 @@ Ltac apply_predicate_equivalence :=
 Add Parametric Morphism i : (glu_univ_elem i)
     with signature glu_typ_pred_equivalence ==> glu_exp_pred_equivalence ==> eq ==> iff as simple_glu_univ_elem_morphism_iff.
 Proof with mautosolve.
-  intros P P' HPP' El El' HElEl' a.
+  intros P P' ? El El'.
   split; intro Horig; [gen El' P' | gen El P];
     induction Horig using glu_univ_elem_ind; unshelve glu_univ_elem_econstructor;
     try (etransitivity; [symmetry + idtac|]; eassumption); eauto.
@@ -489,31 +491,28 @@ Proof.
   handle_per_univ_elem_irrel.
   split; [intros Γ C | intros Γ M C m].
   - split; intros []; econstructor; intuition;
-      rename a0 into c;
-      [rename equiv_a into equiv_c; assert (equiv_c' : in_rel c c) by intuition
-      | rename equiv_a into equiv_c'; assert (equiv_c : in_rel0 c c) by intuition];
+      [rename equiv_m into equiv0_m; assert (equiv_m : in_rel m m) by intuition
+      | assert (equiv0_m : in_rel0 m m) by intuition ];
       destruct_rel_mod_eval;
-      rename a0 into b;
-      assert ((OP c equiv_c' <∙> OP0 c equiv_c) /\ (OEl c equiv_c' <∙> OEl0 c equiv_c)) as [] by mauto 3;
+      functional_eval_rewrite_clear;
+      assert ((OP m equiv_m <∙> OP0 m equiv0_m) /\ (OEl m equiv_m <∙> OEl0 m equiv0_m)) as [] by mauto 3;
       intuition.
   - split; intros []; econstructor; intuition;
-      clear m;
-      rename b into m;
-      [rename equiv_b into equiv_m; assert (equiv_m' : in_rel m m) by intuition
-      | rename equiv_b into equiv_m'; assert (equiv_m : in_rel0 m m) by intuition];
+      [rename equiv_n into equiv0_n; assert (equiv_n : in_rel n n) by intuition
+      | assert (equiv0_n : in_rel0 n n) by intuition];
       destruct_rel_mod_eval;
-      [assert (exists am : domain, {{ $| a0 & m |↘ am }} /\ {{ Δ ⊢ m0[σ] m' : OT[σ,,m'] ® am ∈ OEl m equiv_m' }}) by intuition
-      | assert (exists am : domain, {{ $| a0 & m |↘ am }} /\ {{ Δ ⊢ m0[σ] m' : OT[σ,,m'] ® am ∈ OEl0 m equiv_m }}) by intuition];
+      [assert (exists m0n, {{ $| m0 & n |↘ m0n }} /\ {{ Δ ⊢ M0[σ] N : OT[σ,,N] ® m0n ∈ OEl n equiv_n }}) by intuition
+      | assert (exists m0n, {{ $| m0 & n |↘ m0n }} /\ {{ Δ ⊢ M0[σ] N : OT[σ,,N] ® m0n ∈ OEl0 n equiv0_n }}) by intuition];
       destruct_conjs;
-      assert ((OP m equiv_m' <∙> OP0 m equiv_m) /\ (OEl m equiv_m' <∙> OEl0 m equiv_m)) as [] by mauto 3;
+      assert ((OP n equiv_n <∙> OP0 n equiv0_n) /\ (OEl n equiv_n <∙> OEl0 n equiv0_n)) as [] by mauto 3;
       eexists; split; intuition.
 Qed.
 
 Ltac apply_functional_glu_univ_elem1 :=
   let tactic_error o1 o2 := fail 2 "functional_glu_univ_elem biconditional between" o1 "and" o2 "cannot be solved" in
   match goal with
-  | H1 : {{ DG ~?A ∈ glu_univ_elem ?i ↘ ?P1 ↘ ?El1 }},
-      H2 : {{ DG ~?A ∈ glu_univ_elem ?i' ↘ ?P2 ↘ ?El2 }} |- _ =>
+  | H1 : {{ DG ~?a ∈ glu_univ_elem ?i ↘ ?P1 ↘ ?El1 }},
+      H2 : {{ DG ~?a ∈ glu_univ_elem ?i' ↘ ?P2 ↘ ?El2 }} |- _ =>
       unify i i';
       assert_fails (unify P1 P2; unify El1 El2);
       match goal with
@@ -536,18 +535,18 @@ Ltac handle_functional_glu_univ_elem :=
   apply_predicate_equivalence;
   clear_dups.
 
-Lemma glu_univ_elem_pi_clean_inversion1 : forall {i a p B in_rel typ_rel el_rel},
+Lemma glu_univ_elem_pi_clean_inversion1 : forall {i a ρ B in_rel P El},
   {{ DF a ≈ a ∈ per_univ_elem i ↘ in_rel }} ->
-  {{ DG Π a p B ∈ glu_univ_elem i ↘ typ_rel ↘ el_rel }} ->
+  {{ DG Π a ρ B ∈ glu_univ_elem i ↘ P ↘ El }} ->
   exists IP IEl (OP : forall c (equiv_c_c : {{ Dom c ≈ c ∈ in_rel }}), glu_typ_pred)
      (OEl : forall c (equiv_c_c : {{ Dom c ≈ c ∈ in_rel }}), glu_exp_pred) elem_rel,
       {{ DG a ∈ glu_univ_elem i ↘ IP ↘ IEl }} /\
         (forall c (equiv_c : {{ Dom c ≈ c ∈ in_rel }}) b,
-            {{ ⟦ B ⟧ p ↦ c ↘ b }} ->
+            {{ ⟦ B ⟧ ρ ↦ c ↘ b }} ->
             {{ DG b ∈ glu_univ_elem i ↘ OP _ equiv_c ↘ OEl _ equiv_c }}) /\
-        {{ DF Π a p B ≈ Π a p B ∈ per_univ_elem i ↘ elem_rel }} /\
-        (typ_rel <∙> pi_glu_typ_pred i in_rel IP IEl OP) /\
-        (el_rel <∙> pi_glu_exp_pred i in_rel IP IEl elem_rel OEl).
+        {{ DF Π a ρ B ≈ Π a ρ B ∈ per_univ_elem i ↘ elem_rel }} /\
+        (P <∙> pi_glu_typ_pred i in_rel IP IEl OP) /\
+        (El <∙> pi_glu_exp_pred i in_rel IP IEl elem_rel OEl).
 Proof.
   intros *.
   simpl.
@@ -559,11 +558,11 @@ Proof.
   repeat split.
   1,3: eassumption.
   1: instantiate (1 := fun c equiv_c Γ A M m => forall (b : domain) Pb Elb,
-                          {{ ⟦ B ⟧ p ↦ c ↘ b }} ->
+                          {{ ⟦ B ⟧ ρ ↦ c ↘ b }} ->
                           {{ DG b ∈ glu_univ_elem i ↘ Pb ↘ Elb }} ->
                           {{ Γ ⊢ M : A ® m ∈ Elb }}).
   1: instantiate (1 := fun c equiv_c Γ A => forall (b : domain) Pb Elb,
-                          {{ ⟦ B ⟧ p ↦ c ↘ b }} ->
+                          {{ ⟦ B ⟧ ρ ↦ c ↘ b }} ->
                           {{ DG b ∈ glu_univ_elem i ↘ Pb ↘ Elb }} ->
                           {{ Γ ⊢ A ® Pb }}).
   2-5: intros []; econstructor; mauto.
@@ -575,31 +574,27 @@ Proof.
       split; intros; handle_functional_glu_univ_elem; intuition.
     + intros ? ?.
       split; [intros; handle_functional_glu_univ_elem |]; intuition.
-  - rename a0 into c.
-    rename equiv_a into equiv_c.
-    assert {{ Dom c ≈ c ∈ in_rel0 }} as equiv0_c by intuition.
-    assert {{ DG b ∈ glu_univ_elem i ↘ OP c equiv0_c ↘ OEl c equiv0_c }} by mauto 3.
+  - assert {{ Dom m ≈ m ∈ in_rel0 }} as equiv0_m by intuition.
+    assert {{ DG b ∈ glu_univ_elem i ↘ OP m equiv0_m ↘ OEl m equiv0_m }} by mauto 3.
     handle_functional_glu_univ_elem.
     intuition.
   - match_by_head per_univ_elem ltac:(fun H => directed invert_per_univ_elem H).
     destruct_rel_mod_eval.
     intuition.
-  - rename b into c.
-    rename equiv_b into equiv_c.
-    assert {{ Dom c ≈ c ∈ in_rel0 }} as equiv0_c by intuition.
-    assert (exists ac : domain, {{ $| a0 & c |↘ ac }} /\ {{ Δ ⊢ m[σ] m' : OT[σ,,m'] ® ac ∈ OEl c equiv0_c }}) by mauto 3.
+  - assert {{ Dom n ≈ n ∈ in_rel0 }} as equiv0_n by intuition.
+    assert (exists mn : domain, {{ $| m & n |↘ mn }} /\ {{ Δ ⊢ M[σ] N : OT[σ,,N] ® mn ∈ OEl n equiv0_n }}) by mauto 3.
     destruct_conjs.
     eexists.
     intuition.
-    assert {{ DG b ∈ glu_univ_elem i ↘ OP c equiv0_c ↘ OEl c equiv0_c }} by mauto 3.
+    assert {{ DG b ∈ glu_univ_elem i ↘ OP n equiv0_n ↘ OEl n equiv0_n }} by mauto 3.
     handle_functional_glu_univ_elem.
     intuition.
-  - assert (exists ab : domain,
-               {{ $| a0 & b |↘ ab }} /\
-                 (forall (b0 : domain) (Pb : glu_typ_pred) (Elb : glu_exp_pred),
-                     {{ ⟦ B ⟧ p ↦ b ↘ b0 }} ->
-                     {{ DG b0 ∈ glu_univ_elem i ↘ Pb ↘ Elb }} ->
-                     {{ Δ ⊢ m[σ] m' : OT[σ,,m'] ® ab ∈ Elb }})) by intuition.
+  - assert (exists mn : domain,
+               {{ $| m & n |↘ mn }} /\
+                 (forall (b : domain) (Pb : glu_typ_pred) (Elb : glu_exp_pred),
+                     {{ ⟦ B ⟧ ρ ↦ n ↘ b }} ->
+                     {{ DG b ∈ glu_univ_elem i ↘ Pb ↘ Elb }} ->
+                     {{ Δ ⊢ M[σ] N : OT[σ,,N] ® mn ∈ Elb }})) by intuition.
     destruct_conjs.
     match_by_head per_univ_elem ltac:(fun H => directed invert_per_univ_elem H).
     handle_per_univ_elem_irrel.
@@ -610,18 +605,18 @@ Proof.
     intuition.
 Qed.
 
-Lemma glu_univ_elem_pi_clean_inversion2 : forall {i a p B in_rel IP IEl typ_rel el_rel},
+Lemma glu_univ_elem_pi_clean_inversion2 : forall {i a ρ B in_rel IP IEl P El},
   {{ DF a ≈ a ∈ per_univ_elem i ↘ in_rel }} ->
   {{ DG a ∈ glu_univ_elem i ↘ IP ↘ IEl }} ->
-  {{ DG Π a p B ∈ glu_univ_elem i ↘ typ_rel ↘ el_rel }} ->
+  {{ DG Π a ρ B ∈ glu_univ_elem i ↘ P ↘ El }} ->
   exists (OP : forall c (equiv_c_c : {{ Dom c ≈ c ∈ in_rel }}), glu_typ_pred)
      (OEl : forall c (equiv_c_c : {{ Dom c ≈ c ∈ in_rel }}), glu_exp_pred) elem_rel,
     (forall c (equiv_c : {{ Dom c ≈ c ∈ in_rel }}) b,
-        {{ ⟦ B ⟧ p ↦ c ↘ b }} ->
+        {{ ⟦ B ⟧ ρ ↦ c ↘ b }} ->
         {{ DG b ∈ glu_univ_elem i ↘ OP _ equiv_c ↘ OEl _ equiv_c }}) /\
-      {{ DF Π a p B ≈ Π a p B ∈ per_univ_elem i ↘ elem_rel }} /\
-      (typ_rel <∙> pi_glu_typ_pred i in_rel IP IEl OP) /\
-      (el_rel <∙> pi_glu_exp_pred i in_rel IP IEl elem_rel OEl).
+      {{ DF Π a ρ B ≈ Π a ρ B ∈ per_univ_elem i ↘ elem_rel }} /\
+      (P <∙> pi_glu_typ_pred i in_rel IP IEl OP) /\
+      (El <∙> pi_glu_exp_pred i in_rel IP IEl elem_rel OEl).
 Proof.
   intros *.
   simpl.
@@ -680,7 +675,7 @@ Qed.
 Add Parametric Morphism i R : (glu_univ_elem i)
     with signature glu_typ_pred_equivalence ==> glu_exp_pred_equivalence ==> per_univ_elem i R ==> iff as glu_univ_elem_morphism_iff'.
 Proof with mautosolve.
-  intros P P' HPP' El El' HElEl' a a' Haa'.
+  intros P P' HPP' El El' HElEl' **.
   rewrite HPP', HElEl'.
   split; intros; eapply glu_univ_elem_resp_per_univ; mauto.
   symmetry; mauto.
@@ -717,12 +712,12 @@ Proof.
     + saturate_refl; eassumption.
     + instantiate (1 := fun (c : domain) (equiv_c : in_rel c c) Γ A M m =>
                           forall b P El,
-                            {{ ⟦ B' ⟧ p' ↦ c ↘ b }} ->
+                            {{ ⟦ B' ⟧ ρ' ↦ c ↘ b }} ->
                             glu_univ_elem i P El b ->
                             {{ Γ ⊢ M : A ® m ∈ El }}).
       instantiate (1 := fun (c : domain) (equiv_c : in_rel c c) Γ A =>
                           forall b P El,
-                            {{ ⟦ B' ⟧ p' ↦ c ↘ b }} ->
+                            {{ ⟦ B' ⟧ ρ' ↦ c ↘ b }} ->
                             glu_univ_elem i P El b ->
                             {{ Γ ⊢ A ® P }}).
       intros.
@@ -730,7 +725,7 @@ Proof.
       handle_per_univ_elem_irrel.
       rewrite simple_glu_univ_elem_morphism_iff; try (eassumption + reflexivity);
         split; intros; handle_functional_glu_univ_elem; intuition.
-    + enough {{ DF Π A p B ≈ Π A' p' B' ∈ per_univ_elem i ↘ elem_rel }} by (etransitivity; [symmetry |]; eassumption).
+    + enough {{ DF Π a ρ B ≈ Π a' ρ' B' ∈ per_univ_elem i ↘ elem_rel }} by (etransitivity; [symmetry |]; eassumption).
       per_univ_elem_econstructor; mauto.
       intros.
       (on_all_hyp: destruct_rel_by_assumption in_rel).
@@ -833,23 +828,25 @@ Proof.
       deepexec H1 ltac:(fun H => pose proof H).
       autorewrite with mcltt in *.
       repeat eexists; eauto.
-      assert {{ Δ0 ⊢s σ0,, m' : Δ, ~ (a_sub IT σ) }}. {
+      assert {{ Δ0 ⊢s σ0,,N : Δ, ~ (a_sub IT σ) }}.
+      {
         econstructor; mauto 2.
         bulky_rewrite.
       }
-      assert {{Δ0 ⊢ (m [σ][σ0]) m' ≈ (m [σ ∘ σ0]) m' : OT [σ ∘ σ0,, m']}}. {
+      assert {{Δ0 ⊢ M[σ][σ0] N ≈ M[σ∘σ0] N : OT [σ∘σ0,,N]}}.
+      {
         rewrite <- @sub_eq_q_sigma_id_extend; mauto 4.
         rewrite <- @exp_eq_sub_compose_typ; mauto 3;
           [eapply wf_exp_eq_app_cong' |];
           mauto 4.
         symmetry.
         bulky_rewrite_in H4.
-        assert {{ Δ0 ⊢ Π IT[σ ∘ σ0] (OT[q (σ ∘ σ0)]) ≈ (Π IT OT)[σ ∘ σ0] : Type@(S (max i4 i)) }} by mauto.
+        assert {{ Δ0 ⊢ Π IT[σ∘σ0] (OT[q (σ∘σ0)]) ≈ (Π IT OT)[σ∘σ0] : Type@(S (max i4 i)) }} by mauto.
         eapply wf_exp_eq_conv'; mauto 4.
       }
 
       bulky_rewrite.
-      edestruct H10 with (b := b) as [? []];
+      edestruct H10 with (n := n) as [? []];
         simplify_evals; [| | eassumption];
         mauto.
 
