theories/Core/Soundness/LogicalRelation/CoreTactics.v
@@ -1,5 +1,6 @@
 From Equations Require Import Equations.
 
+From Mcltt Require Import Base LibTactics.
 From Mcltt.Core.Soundness Require Import LogicalRelation.Definitions.
 
 Ltac basic_invert_glu_univ_elem H :=
@@ -12,3 +13,15 @@ Ltac basic_glu_univ_elem_econstructor :=
   progress simp glu_univ_elem;
   econstructor;
   try rewrite <- glu_univ_elem_equation_1 in *.
+
+Ltac invert_glu_rel1 :=
+  match goal with
+  | H : pi_glu_typ_pred _ _ _ _ _ _ _ |- _ =>
+      progressive_invert H
+  | H : pi_glu_exp_pred _ _ _ _ _ _ _ _ _ _ |- _ =>
+      progressive_invert H
+  | H : neut_glu_typ_pred _ _ _ _ |- _ =>
+      progressive_invert H
+  | H : neut_glu_exp_pred _ _ _ _ _ _ |- _ =>
+      progressive_invert H
+  end.
