theories/Core/Soundness/Realizability.v
@@ -8,16 +8,16 @@ Import Domain_Notations.
 
 Open Scope list_scope.
 
-Lemma wf_ctx_sub_ctx_lookup : forall n T Γ,
-    {{ #n : T ∈ Γ }} ->
+Lemma wf_ctx_sub_ctx_lookup : forall n A Γ,
+    {{ #n : A ∈ Γ }} ->
     forall Δ,
       {{ ⊢ Δ ⊆ Γ}} ->
-      exists Δ1 T0 Δ2 T',
-        Δ = Δ1 ++ T0 :: Δ2 /\
+      exists Δ1 A0 Δ2 A',
+        Δ = Δ1 ++ A0 :: Δ2 /\
           n = length Δ1 /\
-          T' = iter (S n) (fun T => {{{T [ Wk ]}}}) T0 /\
-          {{ #n : T' ∈ Δ }} /\
-          {{ Δ ⊢ T' ⊆ T }}.
+          A' = iter (S n) (fun A => {{{ A[Wk] }}}) A0 /\
+          {{ #n : A' ∈ Δ }} /\
+          {{ Δ ⊢ A' ⊆ A }}.
 Proof.
   induction 1; intros; progressive_inversion.
   - exists nil.
@@ -27,9 +27,8 @@ Proof.
     repeat eexists; mauto 4.
 Qed.
 
-
-Lemma var_arith : forall Γ1 Γ2 (T : typ),
-    length (Γ1 ++ T :: Γ2) - length Γ2 - 1 = length Γ1.
+Lemma var_arith : forall Γ1 Γ2 (A : typ),
+    length (Γ1 ++ A :: Γ2) - length Γ2 - 1 = length Γ1.
 Proof.
   intros.
   rewrite List.app_length. simpl.
@@ -38,9 +37,9 @@ Qed.
 
 Lemma var_weaken_gen : forall Δ σ Γ,
     {{ Δ ⊢w σ : Γ }} ->
-    forall Γ1 Γ2 T,
-      Γ = Γ1 ++ T :: Γ2 ->
-      {{Δ ⊢ (# (length Γ1)) [σ] ≈ # (length Δ - length Γ2 - 1) : ~(iter (S (length Γ1)) (fun T => {{{T [ Wk ]}}}) T) [ σ ] }}.
+    forall Γ1 Γ2 A0,
+      Γ = Γ1 ++ A0 :: Γ2 ->
+      {{ Δ ⊢ #(length Γ1)[σ] ≈ #(length Δ - length Γ2 - 1) : ~(iter (S (length Γ1)) (fun A => {{{ A[Wk] }}}) A0)[σ] }}.
 Proof.
   induction 1; intros; subst; gen_presups.
   - pose proof (app_ctx_vlookup _ _ _ _ HΔ eq_refl) as Hvar.
@@ -48,16 +47,16 @@ Proof.
     clear_dups.
     apply wf_sub_id_inversion in Hτ.
     pose proof (wf_ctx_sub_length _ _ Hτ).
-    transitivity {{{#(length Γ1) [Id]}}}; [mauto 3 |].
-    replace (length Γ) with (length (Γ1 ++ {{{ Γ2, T }}})) by eassumption.
+    transitivity {{{ #(length Γ1)[Id] }}}; [mauto 3 |].
+    replace (length Γ) with (length (Γ1 ++ {{{ Γ2, A0 }}})) by eassumption.
     rewrite var_arith, H.
     bulky_rewrite.
   - pose proof (app_ctx_vlookup _ _ _ _ HΔ0 eq_refl) as Hvar.
-    pose proof (app_ctx_lookup Γ1 T0 Γ2 _ eq_refl).
+    pose proof (app_ctx_lookup Γ1 A0 Γ2 _ eq_refl).
     gen_presup Hvar.
     clear_dups.
-    assert {{ ⊢ Δ', T }} by mauto 3.
-    assert {{ Δ', T ⊢s Wk : ~ (Γ1 ++ {{{ Γ2, T0 }}}) }} by mauto 3.
+    assert {{ ⊢ Δ', A }} by mauto 3.
+    assert {{ Δ', A ⊢s Wk : ~ (Γ1 ++ {{{ Γ2, A0 }}}) }} by mauto 3.
     transitivity {{{ #(length Γ1)[Wk∘τ] }}}; [mauto 3 |].
     rewrite H1.
     etransitivity; [eapply wf_exp_eq_sub_compose; mauto 3 |].
@@ -76,16 +75,16 @@ Proof.
       * eapply wf_exp_eq_var_weaken; [mauto 3|]; eauto.
       * mauto 4.
     + eapply wf_exp_eq_subtyp'.
-      * eapply IHweakening with (Γ1 := T :: _).
+      * eapply IHweakening with (Γ1 := A :: _).
         reflexivity.
       * eapply wf_subtyp_subst; [ |mauto 3].
         simpl. eapply wf_subtyp_subst; mauto 3.
 Qed.
 
-Lemma var_glu_elem_bot : forall A i P El Γ T,
-    {{ DG A ∈ glu_univ_elem i ↘ P ↘ El }} ->
-    {{ Γ ⊢ T ® P }} ->
-    {{ Γ, T ⊢ #0 : T[Wk] ® ! (length Γ) ∈ glu_elem_bot i A }}.
+Lemma var_glu_elem_bot : forall a i P El Γ A,
+    {{ DG a ∈ glu_univ_elem i ↘ P ↘ El }} ->
+    {{ Γ ⊢ A ® P }} ->
+    {{ Γ, A ⊢ #0 : A[Wk] ® !(length Γ) ∈ glu_elem_bot i a }}.
 Proof.
   intros. saturate_glu_info.
   econstructor; mauto 4.
@@ -98,19 +97,26 @@ Qed.
 #[local]
 Hint Rewrite -> wf_sub_eq_extend_compose using mauto 4 : mcltt.
 
-Theorem realize_glu_univ_elem_gen : forall A i P El,
-    {{ DG A ∈ glu_univ_elem i ↘ P ↘ El }} ->
-    (forall Γ T R, {{ DF A ≈ A ∈ per_univ_elem i ↘ R }} ->
-              {{ Γ ⊢ T ® P }} ->
-              {{ Γ ⊢ T ® glu_typ_top i A }}) /\
-      (forall Γ t T c, {{ DG A ∈ glu_univ_elem i ↘ P ↘ El }} ->
-                  {{ Γ ⊢ t : T ® c ∈ glu_elem_bot i A }} ->
-                  {{ Γ ⊢ t : T ® ⇑ A c ∈ El }}) /\
-      (forall Γ t T a R, {{ DG A ∈ glu_univ_elem i ↘ P ↘ El }} ->
-                    {{ Γ ⊢ t : T ® a ∈ El }} ->
-                    {{ DF A ≈ A ∈ per_univ_elem i ↘ R }} ->
-                    {{ Dom a ≈ a ∈ R }} ->
-                    {{ Γ ⊢ t : T ® a ∈ glu_elem_top i A }}).
+Theorem realize_glu_univ_elem_gen : forall a i P El,
+    {{ DG a ∈ glu_univ_elem i ↘ P ↘ El }} ->
+    (forall Γ A R,
+        {{ DF a ≈ a ∈ per_univ_elem i ↘ R }} ->
+        {{ Γ ⊢ A ® P }} ->
+        {{ Γ ⊢ A ® glu_typ_top i a }}) /\
+      (forall Γ M A m,
+          (* We repeat this to get the relation between [a] and [P]
+             more easily after applying [induction 1.] *)
+          {{ DG a ∈ glu_univ_elem i ↘ P ↘ El }} ->
+          {{ Γ ⊢ M : A ® m ∈ glu_elem_bot i a }} ->
+          {{ Γ ⊢ M : A ® ⇑ a m ∈ El }}) /\
+      (forall Γ M A m R,
+          (* We repeat this to get the relation between [a] and [P]
+             more easily after applying [induction 1.] *)
+          {{ DG a ∈ glu_univ_elem i ↘ P ↘ El }} ->
+          {{ Γ ⊢ M : A ® m ∈ El }} ->
+          {{ DF a ≈ a ∈ per_univ_elem i ↘ R }} ->
+          {{ Dom m ≈ m ∈ R }} ->
+          {{ Γ ⊢ M : A ® m ∈ glu_elem_top i a }}).
 Proof.
   simpl. induction 1 using glu_univ_elem_ind.
   all:split; [| split]; intros;
@@ -121,7 +127,7 @@ Proof.
     destruct_all.
   - econstructor; eauto; intros.
     progressive_inversion.
-    transitivity {{{Type@j [ σ ]}}}; mauto 4.
+    transitivity {{{ Type@j[σ] }}}; mauto 4.
   - handle_functional_glu_univ_elem.
     match_by_head glu_univ_elem invert_glu_univ_elem.
     clear_dups.
@@ -139,9 +145,8 @@ Proof.
   - deepexec glu_univ_elem_per_univ ltac:(fun H => pose proof H).
     firstorder.
     specialize (H _ _ _ H10) as [? []].
-    econstructor; eauto.
+    econstructor; mauto 3.
     + apply_equiv_left. trivial.
-    + mauto 2.
     + intros.
       saturate_weakening_escape.
       deepexec H ltac:(fun H => destruct H).
@@ -152,7 +157,7 @@ Proof.
 
   - econstructor; eauto; intros.
     progressive_inversion.
-    transitivity {{{ℕ [ σ ]}}}; mauto 3.
+    transitivity {{{ ℕ[σ] }}}; mauto 3.
   - handle_functional_glu_univ_elem.
     match_by_head glu_univ_elem invert_glu_univ_elem.
     apply_equiv_left.
@@ -161,13 +166,12 @@ Proof.
 
     intros.
     saturate_weakening_escape.
-    assert {{ Δ ⊢ T [σ] ≈ ℕ[σ] : Type @ i }} by mauto 3.
+    assert {{ Δ ⊢ A[σ] ≈ ℕ[σ] : Type @ i }} by mauto 3.
     rewrite <- wf_exp_eq_nat_sub; try eassumption.
     mauto 3.
-  - econstructor; eauto.
-    + rewrite H2. mauto 3.
+  - econstructor; mauto 3.
+    + bulky_rewrite. mauto 3.
     + apply_equiv_left. trivial.
-    + mauto 2.
     + intros.
       saturate_weakening_escape.
       bulky_rewrite.
@@ -180,23 +184,23 @@ Proof.
     + gen_presups. trivial.
     + saturate_weakening_escape.
       assert {{ Γ ⊢w Id : Γ }} by mauto 4.
-      pose proof (H13 _ _ H16).
-      specialize (H13 _ _ H19).
-      assert {{ Γ ⊢ IT[Id] ≈ IT : Type@i}} by mauto 3.
-      bulky_rewrite_in H13.
-      progressive_invert H17.
-      destruct (H9 _ _ _ H0 H13) as [].
+      assert {{ Δ ⊢ IT[σ] ® IP }} by mauto 3.
+      assert (IP Γ {{{ IT[Id] }}}) as HITId by mauto 3.
+      bulky_rewrite_in HITId.
+      assert {{ Γ ⊢ IT[Id] ≈ IT : Type@i }} by mauto 3.
+      dir_inversion_clear_by_head read_typ.
+      assert {{ Γ ⊢ IT ® glu_typ_top i a }} as [] by mauto 3.
       bulky_rewrite.
       simpl. apply wf_exp_eq_pi_cong'; [firstorder |].
       pose proof (var_per_elem (length Δ) H0).
       destruct_rel_mod_eval.
       simplify_evals.
       destruct (H2 _ ltac:(eassumption) _ ltac:(eassumption)) as [? []].
-      specialize (H10 _ _ _ _ ltac:(trivial) (var_glu_elem_bot _ _ _ _ _ _ ltac:(eassumption) ltac:(eassumption))).
-      autorewrite with mcltt in H10.
-      specialize (H14 {{{Δ, IT[σ]}}} {{{σ ∘ Wk}}} _ _ ltac:(mauto) ltac:(eassumption) ltac:(eassumption)).
+      assert (IEl {{{ Δ, IT[σ] }}} {{{ IT[σ][Wk] }}} {{{ #0 }}} d{{{ ⇑! a (length Δ) }}}) by mauto 3 using var_glu_elem_bot.
+      autorewrite with mcltt in H31.
+      specialize (H14 {{{ Δ, IT[σ] }}} {{{ σ∘Wk }}} _ _ ltac:(mauto) ltac:(eassumption) ltac:(eassumption)).
       specialize (H8 _ _ _ ltac:(eassumption) ltac:(eassumption)) as [].
-      etransitivity; [| eapply H30]; mauto 3.
+      etransitivity; [| eapply H33]; mauto 3.
   - handle_functional_glu_univ_elem.
     apply_equiv_left.
     invert_glu_rel1.
@@ -210,18 +214,18 @@ Proof.
     simplify_evals.
     eexists; repeat split; mauto 3.
     eapply H2; eauto.
-    assert {{ Δ ⊢ t [σ] : M[σ] }} by mauto 3.
+    assert {{ Δ ⊢ M[σ] : A[σ] }} by mauto 3.
     bulky_rewrite_in H23.
     unshelve (econstructor; eauto).
     + trivial.
-    + eassert {{ Δ ⊢ ~ (a_sub t σ) m' : ~_ }} by (eapply wf_app'; eassumption).
+    + eassert {{ Δ ⊢ M[σ] N : ~_ }} by (eapply wf_app'; eassumption).
       autorewrite with mcltt in H25.
       trivial.
     + mauto using domain_app_per.
     + intros.
       saturate_weakening_escape.
       progressive_invert H26.
-      destruct (H15 _ _ _ _ _ ltac:(eassumption) ltac:(eassumption) ltac:(eassumption) equiv_b).
+      destruct (H15 _ _ _ _ _ ltac:(eassumption) ltac:(eassumption) ltac:(eassumption) equiv_n).
       handle_functional_glu_univ_elem.
       autorewrite with mcltt.
 
@@ -232,7 +236,7 @@ Proof.
         rewrite <- @exp_eq_sub_compose_typ; mauto 3;
           [eapply wf_exp_eq_app_cong' |].
         -- specialize (H12 _ {{{σ ∘ σ0}}} _ ltac:(mauto 3) ltac:(eassumption)).
-           rewrite wf_exp_eq_sub_compose with (M := t) in H12; mauto 3.
+           rewrite wf_exp_eq_sub_compose with (M := M) in H12; mauto 3.
            bulky_rewrite_in H12.
         -- rewrite <- @exp_eq_sub_compose_typ; mauto 3.
         -- econstructor; mauto 3.
@@ -254,15 +258,15 @@ Proof.
       assert {{ Γ ⊢w Id : Γ }} by mauto 4.
       pose proof (H10 _ _ H24).
       specialize (H10 _ _ H19).
-      assert {{ Γ ⊢ IT[Id] ≈ IT : Type@i}} by mauto 3.
+      assert {{ Γ ⊢ IT[Id] ≈ IT : Type@i }} by mauto 3.
       bulky_rewrite_in H25.
       destruct (H11 _ _ _ ltac:(eassumption) ltac:(eassumption)) as [].
       specialize (H29 _ _ _ H19 H9).
       rewrite H5 in *.
       autorewrite with mcltt.
-      eassert {{ Δ ⊢ m[σ] : ~_ }} by (mauto 2).
+      eassert {{ Δ ⊢ M[σ] : ~_ }} by (mauto 2).
       autorewrite with mcltt in H30.
-      rewrite @wf_exp_eq_pi_eta' with (M := {{{m[σ]}}}); [| trivial].
+      rewrite @wf_exp_eq_pi_eta' with (M := {{{ M[σ] }}}); [| trivial].
       cbn [nf_to_exp].
       eapply wf_exp_eq_fn_cong'; eauto.
 
@@ -282,7 +286,7 @@ Proof.
       do 2 (rewrite wf_exp_eq_sub_id in H40; mauto 3).
       etransitivity; [|eassumption].
       simpl.
-      assert {{ Δ, IT[σ] ⊢ # 0 : IT[σ ∘ Wk] }} by (rewrite <- @exp_eq_sub_compose_typ; mauto 3).
+      assert {{ Δ, IT[σ] ⊢ #0 : IT[σ∘Wk] }} by (rewrite <- @exp_eq_sub_compose_typ; mauto 3).
       rewrite <- @sub_eq_q_sigma_id_extend; mauto 4.
       rewrite <- @exp_eq_sub_compose_typ; mauto 2.
       2:eapply sub_q; mauto 4.
@@ -309,12 +313,11 @@ Proof.
       firstorder.
 Qed.
 
-
-Corollary realize_glu_typ_top : forall A i P El,
-    {{ DG A ∈ glu_univ_elem i ↘ P ↘ El }} ->
-    forall Γ T,
-      {{ Γ ⊢ T ® P }} ->
-      {{ Γ ⊢ T ® glu_typ_top i A }}.
+Corollary realize_glu_typ_top : forall a i P El,
+    {{ DG a ∈ glu_univ_elem i ↘ P ↘ El }} ->
+    forall Γ A,
+      {{ Γ ⊢ A ® P }} ->
+      {{ Γ ⊢ A ® glu_typ_top i a }}.
 Proof.
   intros.
   pose proof H.
@@ -323,21 +326,21 @@ Proof.
   eapply realize_glu_univ_elem_gen; eauto.
 Qed.
 
-Theorem realize_glu_elem_bot : forall A i P El,
-    {{ DG A ∈ glu_univ_elem i ↘ P ↘ El }} ->
-    forall Γ t T c,
-      {{ Γ ⊢ t : T ® c ∈ glu_elem_bot i A }} ->
-      {{ Γ ⊢ t : T ® ⇑ A c ∈ El }}.
+Theorem realize_glu_elem_bot : forall a i P El,
+    {{ DG a ∈ glu_univ_elem i ↘ P ↘ El }} ->
+    forall Γ A M m,
+      {{ Γ ⊢ M : A ® m ∈ glu_elem_bot i a }} ->
+      {{ Γ ⊢ M : A ® ⇑ a m ∈ El }}.
 Proof.
   intros.
   eapply realize_glu_univ_elem_gen; eauto.
 Qed.
 
-Theorem realize_glu_elem_top : forall A i P El,
-    {{ DG A ∈ glu_univ_elem i ↘ P ↘ El }} ->
-    forall Γ t T a,
-      {{ Γ ⊢ t : T ® a ∈ El }} ->
-      {{ Γ ⊢ t : T ® a ∈ glu_elem_top i A }}.
+Theorem realize_glu_elem_top : forall a i P El,
+    {{ DG a ∈ glu_univ_elem i ↘ P ↘ El }} ->
+    forall Γ A M m,
+      {{ Γ ⊢ M : A ® m ∈ El }} ->
+      {{ Γ ⊢ M : A ® m ∈ glu_elem_top i a }}.
 Proof.
   intros.
   pose proof H.
